Wavelet/Dataflow/EqMod.lean
@@ -1,0 +1,68 @@
+import Wavelet.Dataflow.Proc
+
+namespace Wavelet.Dataflow
+
+open Semantics
+
+/-- Checks if two channel maps are equal modulo an equivalence relation on values. -/
+def ChanMap.EqMod
+  (Eq : V → V → Prop)
+  (map₁ map₂ : ChanMap χ V) : Prop :=
+  ∀ {name : χ}, List.Forall₂ Eq (map₁ name) (map₂ name)
+
+instance {Eq : V → V → Prop} [IsRefl V Eq] : IsRefl (ChanMap χ V) (ChanMap.EqMod Eq) where
+  refl map := by
+    intros name
+    apply List.forall₂_refl
+
+@[simp]
+theorem ChanMap.EqMod.eq_eq {map₁ map₂ : ChanMap χ V} :
+    ChanMap.EqMod Eq map₁ map₂ ↔ map₁ = map₂
+  := by
+  constructor
+  · simp [EqMod]
+    intros h
+    funext
+    apply h
+  · intros h
+    simp [h, EqMod]
+
+/-- Equal configurations modulo a equivalence relation on values. -/
+def Config.EqMod
+  [Arity Op] (Eq : V → V → Prop)
+  (c₁ c₂ : Config Op χ V m n) : Prop :=
+  c₁.proc = c₂.proc ∧
+  ChanMap.EqMod Eq c₁.chans c₂.chans
+
+instance {Eq : V → V → Prop} [Arity Op] [IsRefl V Eq] :
+  IsRefl (Config Op χ V m n) (Config.EqMod Eq) where
+  refl c := by
+    constructor
+    · rfl
+    · apply IsRefl.refl
+
+instance {Eq : V → V → Prop} [Arity Op] [IsTrans V Eq] :
+  IsTrans (Config Op χ V m n) (Config.EqMod Eq) where
+  trans := sorry
+
+@[simp]
+theorem Config.EqMod.eq_eq
+  [Arity Op] {c₁ c₂ : Config Op χ V m n} :
+    Config.EqMod Eq c₁ c₂ ↔ c₁ = c₂
+  := by
+  simp [EqMod]
+  cases c₁; cases c₂
+  simp
+
+theorem chan_map_push_vals_equiv
+  [DecidableEq χ]
+  {map : ChanMap χ V}
+  {vals₁ vals₂ : Vector V k}
+  {Eq : V → V → Prop}
+  (hequiv : List.Forall₂ Eq vals₁.toList vals₂.toList) :
+    ChanMap.EqMod EqV
+      (ChanMap.pushVals names vals₁ map)
+      (ChanMap.pushVals names vals₂ map)
+  := sorry
+
+end Wavelet.Dataflow
